util/Utils.v
@@ -3,6 +3,10 @@ Set Implicit Arguments.
 Unset Strict Implicit.
 
 Require Import PeanoNat.
+Require Import Coq.Numbers.Cyclic.Int63.Uint63.
+Require Import List.
+
+Coercion is_true b := b = true.
 
 Lemma eta_pair {A B} (p : A * B) : p = (fst p, snd p).
 Proof. destruct p; trivial. Qed.
@@ -17,3 +21,32 @@ Proof.
       rewrite PeanoNat.Nat.lt_succ_r in LT.
       apply (PeanoNat.Nat.lt_le_trans _ _ _ LT' LT).
 Defined.
+
+Lemma negb_lt_le x h : negb (x <? h)%uint63 -> (h <=? x)%uint63.
+Proof.
+    destruct (ltbP x h) as [|B]; try discriminate.
+    apply BinInt.Z.nlt_ge in B.
+    rewrite <- leb_spec in B; trivial.
+Qed.
+
+Lemma negb_lt_x_x x : negb (x <? x)%uint63.
+Proof. unfold is_true. destruct (ltbP x x) as [|B]; auto with *. Qed.
+
+Lemma lt_le x h : (x <? h)%uint63 -> (x <=? h)%uint63.
+Proof.
+    destruct (ltbP x h) as [|B]; try discriminate.
+    intros _. unfold is_true. rewrite leb_spec.
+    apply BinInt.Z.lt_le_incl; trivial.
+Qed.
+
+Lemma leb_trans x h i : (x <=? h)%uint63 -> (h <=? i)%uint63 -> (x <=? i)%uint63.
+Proof.
+  intros E1 E2. unfold is_true in *. rewrite leb_spec in *.
+  apply (BinInt.Z.le_trans _ _ _ E1 E2).
+Qed.
+
+Lemma In_middle A l (x : A) r : In x (l ++ x :: r).
+Proof. apply in_or_app; auto with *. Qed.
+
+Definition All {A : Type} (P : A -> Prop) (l : list A) : Prop :=
+  forall x, In x l -> P x.
